steel/Zeta.Steel.VerifierTypes.fsti
@@ -57,3 +57,52 @@ let extract_tsm_entries_invariant (#o:_) (#tsm:M.thread_state_model) (t:thread_s
       tsm_entries_invariant tsm)
   = elim_thread_state_inv t;
     intro_thread_state_inv t
+
+noeq
+type kv = {
+     key:key;
+     value:(v:value {is_value_of key v})
+}
+
+module U16 = FStar.UInt16
+inline_for_extraction
+let read_store_t =
+    #tsm:M.thread_state_model ->
+    t:thread_state_t ->
+    slot:slot ->
+    ST (option kv)
+       (thread_state_inv t tsm)
+       (fun _ -> thread_state_inv t tsm)
+       (requires True)
+       (ensures fun o ->
+         match Seq.index tsm.store (U16.v slot), o with
+         | None, None -> True
+         | Some (se : M.store_entry), Some kv -> se.key == kv.key /\ se.value == kv.value
+         | _ -> False)
+
+
+let value_compat_with_slot (tsm:M.thread_state_model) (slot:slot) (v:value)
+  : prop
+  = match Seq.index tsm.store (U16.v slot) with
+    | None -> False
+    | Some (se : M.store_entry) -> is_value_of se.key v == true
+
+let update_tsm_slot_value (tsm:M.thread_state_model) (slot:slot) (v:value { value_compat_with_slot tsm slot v })
+  : GTot M.thread_state_model
+  = let Some se = Seq.index tsm.store (U16.v slot) in
+    let se' = { se with value = v } in
+    let store' = Seq.upd tsm.store (U16.v slot) (Some se') in
+    { tsm with store = store' }
+
+inline_for_extraction
+let write_store_t =
+    #tsm:M.thread_state_model ->
+    t:thread_state_t ->
+    slot:slot ->
+    v:value { value_compat_with_slot tsm slot v } ->
+    STT unit
+       (thread_state_inv_core t tsm)
+       (fun _ -> thread_state_inv_core t (update_tsm_slot_value tsm slot v))
+
+val read_store : read_store_t
+val write_store : write_store_t
